theories/base.v
@@ -217,6 +217,18 @@ Section map_filter_lookup.
     (∀ x, m !! i = Some x → P (i, x)) → filter P m !! i = m !! i.
   Proof. move => ?. rewrite map_filter_lookup. destruct (m !! i) => //=. case_option_guard; naive_solver. Qed.
 End map_filter_lookup.
+Section theorems.
+Context `{FinMap K M}.
+Section map_filter.
+  Context {A} (P : K * A → Prop) `{!∀ x, Decision (P x)}.
+  Implicit Types m : M A.
+
+  Lemma map_filter_empty_iff_2 m :
+    map_Forall (λ i x, ¬P (i,x)) m →
+    filter P m = ∅.
+  Proof. apply map_filter_empty_iff. Qed.
+End map_filter.
+End theorems.
 
 Section dom.
 Context `{FinMapDom K M D}.
