theories/imp_to_asm_examples.v
@@ -150,17 +150,25 @@ Lemma asm_add_refines_imp_add :
            (MS (imp_to_asm (dom _ asm_add) (dom _ imp_add_prog) (<["add" := 100]> ∅) imp_module) (initial_imp_to_asm_state imp_module (initial_imp_state imp_add_prog))).
 Proof.
   apply imp_to_asm_proof; [set_solver..|].
-  move => n i rs mem K f fn avs vs h cs pc ret ra r amem ih Hpc Hi Hf Hf2i Hvalid Hinv ? Hmem Hargs ? Hcall Hret.
+  move => n i rs mem K f fn avs vs h cs pc ret rf rc amem ih Hpc Hi Hf Hf2i Hsat Hinv Hargs ? Hcall Hret.
   unfold imp_add_prog in Hf. unfold asm_add in Hi.
   move: Hf2i. rewrite !lookup_insert_Some => ?; destruct_all?; simplify_map_eq/=.
   destruct vs as [|v1 [|v2 []]] => //=.
-  move: Hargs => -[?[? /= [??]]]. decompose_Forall_hyps.
+  move: Hargs => -[?[? /= [??]]].
+  iSatStart. iIntros!.
+  iDestruct (big_sepL2_cons_inv_l with "[$]") as (???) "[??]".
+  iDestruct (big_sepL2_cons_inv_l with "[$]") as (???) "[??]".
+  iDestruct (big_sepL2_nil_inv_l with "[$]") as %?. simplify_eq/=. decompose_Forall_hyps.
+  iSatStop.
   tstep_i. split; [simplify_map_eq'|].
   tstep_i; simplify_map_eq'. split; [done|].
   tstep_i => ??. simplify_map_eq'.
   tstep_i; simplify_map_eq'. split!.
   go_s => n1 n2 ??; subst.
-  apply: Hret. 1: by simplify_map_eq. 1: done. 1: by simplify_map_eq'. 1: done. 1: done.
+  iSatStart. simpl. iDestruct!. iSatStop.
+  apply: Hret. 1: by simplify_map_eq.
+  1: { iSatMono. iFrame. done. }
+  1: by simplify_map_eq'.
   1: { unfold imp_to_asm_ret; split!; simplify_map_eq' => //. }
   1: by simplify_map_eq'.
 Qed.
@@ -172,11 +180,14 @@ Lemma asm_add_client_refines_imp_add_client :
                (initial_imp_to_asm_state imp_module (initial_imp_state imp_add_client_prog) )).
 Proof.
   apply imp_to_asm_proof; [set_solver..|].
-  move => n i rs mem K f fn avs vs h cs pc ret ra r amem ih Hpc Hi Hf Hf2i Hvalid Hinv ? Hmem Hargs ? Hcall Hret.
+  move => n i rs mem K f fn avs vs h cs pc ret rf rc amem ih Hpc Hi Hf Hf2i Hsat [Hmem [Hheap Hsp]] Hargs ? Hcall Hret.
   unfold imp_add_client_prog in Hf. unfold asm_add_client in Hi.
   move: Hf2i. rewrite !lookup_insert_Some => ?; destruct_all?; simplify_map_eq/=.
   destruct vs as [|] => //=.
-  move: Hargs => -[?[? /= [? ?]]]. decompose_Forall_hyps.
+  move: Hargs => -[?[? /= [? ?]]].
+  iSatStart. iIntros!.
+  iDestruct (big_sepL2_nil_inv_l with "[$]") as %?. simplify_eq/=. decompose_Forall_hyps.
+  iSatStop.
   tstep_i. split; [simplify_map_eq'|].
   tstep_i; simplify_map_eq'. split; [done|].
   tstep_i => ??. simplify_map_eq'.
@@ -200,10 +211,27 @@ Proof.
   tstep_s.
   change (imp.Call "add" [Val 1; Val 1]) with (expr_fill [] (imp.Call "add" [Val 1; Val 1])).
   apply: Hcall. { repeat econs. } { by simplify_map_eq. } { set_solver. } { set_solver. } { by simplify_map_eq. }
-  { done. } { simplify_map_eq'. admit. } { repeat econs. } { admit. }
+  { iSatMonoBupd.
+    iRename select (i2a_heap_shared_agree _ _) into "Hag".
+    iMod (i2a_mem_alloc (rs !!! "SP" - 1) with "[$]") as "[??]"; [apply Hsp; lia|].
+    iModIntro.
+    iFrame. iSplitL "Hag".
+    { rewrite heap_free_update // heap_free_alloc //=. rewrite left_id_L. apply is_fresh. }
+    iSplitR; [|iDestruct!; iAccu].
+    instantiate (1 := [_;_]) => /=. done.
+  }
+  { split_and!.
+    - move => ?? /lookup_insert_Some?. destruct_all?; simplify_map_eq' => //. by apply Hmem.
+    - split. { apply union_subseteq_r'. apply Hheap. }
+      move => l ??. etrans; [|by eapply Hheap].
+      rewrite heap_free_update // heap_free_alloc //=.
+      rewrite left_id_L. apply is_fresh.
+    - simplify_map_eq'. move => ??. apply lookup_insert_None. split; [|lia]. apply Hsp. lia.
+  }
   { unfold imp_to_asm_args. split!; decompose_Forall; by simplify_map_eq'. }
   { by simplify_map_eq. } { by simplify_map_eq'. }
-  move => rs'' mem'' av v h'' amem'' ih'' rv'' Hpc'' Hvalid'' Hinv'' Hv Hmem'' Hr.
+  iSatClear.
+  move => rs'' mem'' av v h'' amem'' ih'' rf'' Hpc'' Hsat'' [Hmem'' [Hheap'' Hsp'']] Hr.
   move: Hr => [?[? Hm]]; simplify_map_eq'.
   tstep_i; simplify_map_eq'. split!; [by simplify_map_eq'..|].
   tstep_i; simplify_map_eq'. split!; [done..|].
@@ -211,17 +239,26 @@ Proof.
   tstep_i => ??. simplify_map_eq'.
   have ->: rs !!! "SP" - 1 + 1 = rs !!! "SP" by lia.
   tstep_i; simplify_map_eq'. split; [done|].
+  iSatStart. iIntros!.
+  iDestruct (i2a_mem_lookup with "[$] [$]") as %?.
+  iSatStop.
   apply: Hret.
-  1: { simplify_map_eq'. admit. }
-  1: done.
-  1: { simplify_map_eq'. admit. }
-  1: done.
-  1: { admit. }
-  2 : { move => ?. simplify_map_eq' => ?. admit.
-        (* etrans; [eapply Hmem; simplify_map_eq'; lia|]. rewrite lookup_total_insert_ne //. lia. *)
+  1: { simplify_map_eq'. f_equal. by apply: Hmem''. }
+  1: { iSatMonoBupd.
+       iMod (i2a_mem_delete with "[$]") as "?".
+       iModIntro.
+       iFrame.
+  }
+  { split_and!.
+    - move => ?? /lookup_delete_Some?. destruct_all?; simplify_map_eq' => //. by apply Hmem''.
+    - done.
+    - simplify_map_eq'. move => a ?. apply lookup_delete_None.
+      destruct (decide (rs !!! "SP" - 1 = a)); [lia|].
+      right. apply Hsp''. simplify_map_eq'. lia.
   }
   1: { unfold imp_to_asm_ret; split!; simplify_map_eq'; split!. apply lookup_lookup_total; simplify_map_eq'. }
-Admitted.
+  1: { by simplify_map_eq'. }
+Qed.
 
 (*
 The following does not actually hold since the allocation adds a new provenance to h_heap provs
